

$$x_2 = x_1 + \Delta x_{fr} \frac{p_1 - p_0}{p_1},$$

$$p_{y2} = p_{y1} + y_1 \frac{\Delta y_{fr} - \Delta y_{fra} y_1^2}{p_1^2},$$

$$z_2 = z_1 + \frac{\Delta x_{fr} p_{x1} + (\Delta y_{fr} - \Delta y_{fra} y_1^2 / 2) y_1^2 / (2 p_1)}{p_1},$$

$$\text{where } \Delta x_{fr} \equiv \frac{F1^2}{24\rho_b},$$

$$\Delta y_{fr} \equiv \frac{F1}{6\rho_b^2}, \tag{95}$$

$$\Delta y_{fra} \equiv \frac{2}{3} \frac{1}{F1\rho_b^2},$$

$$\rho_b \equiv \frac{L'}{\text{ANGLE} + K0},$$

$$L' \equiv L - \frac{(\text{ANGLE } F1)^2}{24L} \\ \times \frac{\sin((\text{ANGLE}(1 - E1 - E2) - AE1 - AE2)/2)}{\sin(\text{ANGLE}/2)}.$$